Ed25519: Start proving correctness of sign_steps

code/experimental/ed25519/Hacl.Impl.Ed25519.Sign.Steps.fst
@@ -34,12 +34,16 @@ val point_mul_g_compress:
   Stack unit
     (requires fun h ->
       live h out /\ live h s /\ disjoint s out)
-    (ensures fun h0 _ h1 -> modifies (loc out) h0 h1)
+    (ensures fun h0 _ h1 -> modifies (loc out) h0 h1 /\
+      as_seq h1 out == Spec.Ed25519.point_compress (Spec.Ed25519.point_mul (as_seq h0 s) Spec.Ed25519.g)
+    )
+
 let point_mul_g_compress out s =
   push_frame();
   let tmp:point = create 20ul (u64 0) in
   Hacl.Impl.Ed25519.Ladder.point_mul_g tmp s;
   Hacl.Impl.Ed25519.PointCompress.point_compress out tmp;
+  admit();
   pop_frame()
 
 val sign_step_1:
@@ -60,7 +64,6 @@ let sign_step_1 secret tmp_bytes =
   let apre   = sub tmp_bytes 224ul 64ul in
   let a      = sub apre 0ul 32ul in
   let prefix = sub apre 32ul 32ul in
-  admit();
   Hacl.Impl.Ed25519.SecretExpand.secret_expand apre secret;
   point_mul_g_compress a'' a
 
@@ -84,8 +87,39 @@ let sign_step_2 len msg tmp_bytes tmp_ints =
   let apre   = sub tmp_bytes 224ul 64ul in
   let a      = sub apre 0ul 32ul in
   let prefix = sub apre 32ul 32ul in
-  admit();
   Hacl.Impl.SHA512.ModQ.sha512_modq_pre r prefix len msg
+
+val sign_step_3:
+    tmp_bytes:lbuffer uint8 352ul
+  -> tmp_ints:lbuffer uint64 65ul ->
+  Stack unit
+    (requires fun h ->
+      live h tmp_bytes /\ live h tmp_ints /\ disjoint tmp_bytes tmp_ints /\
+      nat_from_intseq_le (as_seq h (gsub tmp_ints 20ul 5ul)) < pow2 256)
+    (ensures fun h0 _ h1 -> modifies (loc tmp_bytes) h0 h1 /\
+      // Framing
+      as_seq h0 (gsub tmp_bytes 96ul 32ul) == as_seq h1 (gsub tmp_bytes 96ul 32ul) /\
+      as_seq h0 (gsub tmp_bytes 224ul 32ul) == as_seq h1 (gsub tmp_bytes 224ul 32ul) /\
+      // Postcondition
+      as_seq h1 (gsub tmp_bytes 160ul 32ul) ==
+      Spec.Ed25519.point_compress (Spec.Ed25519.point_mul
+        (nat_to_bytes_le 32 (nat_from_intseq_le (as_seq h0 (gsub tmp_ints 20ul 5ul))))
+        (Spec.Ed25519.g)))
+
+let sign_step_3 tmp_bytes tmp_ints =
+  let a''  = sub tmp_bytes 96ul  32ul in
+  let apre = sub tmp_bytes 224ul 64ul in
+  let a    = sub apre 0ul 32ul in
+  push_frame();
+  let rb = create 32ul (u8 0) in
+  let r  = sub tmp_ints 20ul 5ul  in
+  let rs' = sub tmp_bytes 160ul 32ul in
+  let h0 = ST.get() in
+  Hacl.Impl.Store56.store_56 rb r;
+  let h1 = ST.get() in
+  assume (as_seq h1 rb == (nat_to_bytes_le 32 (nat_from_intseq_le (as_seq h0 (gsub tmp_ints 20ul 5ul)))));
+  point_mul_g_compress rs' rb;
+  pop_frame()
 
 val sign_step_4:
     len:size_t{v len + 64 <= max_size_t}
@@ -122,36 +156,6 @@ let sign_step_4 len msg tmp_bytes tmp_ints =
   let a    = sub apre 0ul 32ul in
   admit();
   Hacl.Impl.SHA512.ModQ.sha512_modq_pre_pre2 h rs' a'' len msg
-
-val sign_step_3:
-    tmp_bytes:lbuffer uint8 352ul
-  -> tmp_ints:lbuffer uint64 65ul ->
-  Stack unit
-    (requires fun h ->
-      live h tmp_bytes /\ live h tmp_ints /\ disjoint tmp_bytes tmp_ints /\
-      nat_from_intseq_le (as_seq h (gsub tmp_ints 20ul 5ul)) < pow2 256)
-    (ensures fun h0 _ h1 -> modifies (loc tmp_bytes) h0 h1 /\
-      // Framing
-      as_seq h0 (gsub tmp_bytes 96ul 32ul) == as_seq h1 (gsub tmp_bytes 96ul 32ul) /\
-      as_seq h0 (gsub tmp_bytes 224ul 32ul) == as_seq h1 (gsub tmp_bytes 224ul 32ul) /\
-      // Postcondition
-      as_seq h1 (gsub tmp_bytes 160ul 32ul) ==
-      Spec.Ed25519.point_compress (Spec.Ed25519.point_mul
-        (nat_to_bytes_le 32 (nat_from_intseq_le (as_seq h0 (gsub tmp_ints 20ul 5ul))))
-        (Spec.Ed25519.g)))
-
-let sign_step_3 tmp_bytes tmp_ints =
-  let a''  = sub tmp_bytes 96ul  32ul in
-  let apre = sub tmp_bytes 224ul 64ul in
-  let a    = sub apre 0ul 32ul in
-  push_frame();
-  let rb = create 32ul (u8 0) in
-  let r  = sub tmp_ints 20ul 5ul  in
-  let rs' = sub tmp_bytes 160ul 32ul in
-  Hacl.Impl.Store56.store_56 rb r;
-  point_mul_g_compress rs' rb;
-  admit();
-  pop_frame()
 
 val sign_step_5:
     tmp_bytes:lbuffer uint8 352ul
